pulse/lib/pulse/lib/Pulse.Lib.PCM.FractionalPreorder.fst
@@ -1,0 +1,108 @@
+(*
+   Copyright 2024 Microsoft Research
+
+   Licensed under the Apache License, Version 2.0 (the "License");
+   you may not use this file except in compliance with the License.
+   You may obtain a copy of the License at
+
+       http://www.apache.org/licenses/LICENSE-2.0
+
+   Unless required by applicable law or agreed to in writing, software
+   distributed under the License is distributed on an "AS IS" BASIS,
+   WITHOUT WARRANTIES OR CONDITIONS OF ANY KIND, either express or implied.
+   See the License for the specific language governing permissions and
+   limitations under the License.
+*)
+
+module Pulse.Lib.PCM.FractionalPreorder
+
+open FStar.PCM
+open FStar.Preorder
+open PulseCore.Preorder
+open PulseCore.FractionalPermission
+
+module L = FStar.List.Tot
+
+type pcm_carrier (#a:Type u#a) (p:preorder a) : Type u#a = option perm & hist p
+
+let pcm_composable (#a:Type) (p:preorder a) : symrel (pcm_carrier p) =
+  fun x0 x1 ->
+  match x0, x1 with
+  | (None, t0), (None, t1) -> t0 `extends` t1 \/ t1 `extends` t0
+  | (Some _, t0), (None, t1) -> t0 `extends` t1
+  | (None, t0), (Some _, t1) -> t1 `extends` t0
+  | (Some p0, t0), (Some p1, t1) ->
+    t0 == t1 /\
+    sum_perm p0 p1 `lesser_equal_perm` full_perm
+
+let pcm_op (#a:Type) (p:preorder a)
+  (x:pcm_carrier p)
+  (y:pcm_carrier p { pcm_composable p x y })
+  : pcm_carrier p =
+
+  match x, y with
+  | (None, t0), (None, t1) -> None, p_op p t0 t1
+  | (Some _, _), (None, _) -> x
+  | (None, _), (Some _, _) -> y
+  | (Some p0, t0), (Some p1, t1) -> Some (sum_perm p0 p1), t0
+
+let pcm_one (#a:Type) (p:preorder a) : pcm_carrier p = None, []
+
+let fp_pcm' (#a:Type) (p:preorder a) : pcm' (pcm_carrier p) = {
+  composable = pcm_composable p;
+  op = pcm_op p;
+  one = pcm_one p;
+}
+
+let fp_lem_commutative (#a:Type) (p:preorder a) : lem_commutative (fp_pcm' p) =
+  fun _ _ -> ()
+
+let fp_lem_assoc_l (#a:Type) (p:preorder a) : lem_assoc_l (fp_pcm' p) =
+  fun _ _ _ -> ()
+
+#push-options "--z3rlimit_factor 4"
+let fp_lem_assoc_r (#a:Type) (p:preorder a) : lem_assoc_r (fp_pcm' p) =
+  fun _ _ _ -> ()
+#pop-options
+
+let rec extends_nil (#a:Type) (#p:preorder a) (l:hist p)
+  : Lemma (l `extends` []) =
+
+  match l with
+  | [] -> ()
+  | _::tl -> extends_nil #a #p tl
+
+let fp_lem_is_unit (#a:Type) (p:preorder a) : FStar.PCM.lem_is_unit (fp_pcm' p) =
+  fun x ->
+  match x with
+  | Some _, t -> extends_nil t
+  | None, t -> p_op_nil p t
+
+let fp_pcm (#a:Type) (p:preorder a) : pcm (pcm_carrier p) = {
+  p = fp_pcm' p;
+  comm = fp_lem_commutative p;
+  assoc = fp_lem_assoc_l p;
+  assoc_r = fp_lem_assoc_r p;
+  is_unit = fp_lem_is_unit p;
+  refine = (fun _ -> True);
+}
+
+let mk_frame_preserving_upd (#a:Type) (p:preorder a)
+  (t0:hist p) (v:a { qhistory p (v::t0) })
+  : frame_preserving_upd (fp_pcm p) (Some full_perm, t0) (Some full_perm, v::t0) =
+  fun _ -> Some full_perm, v::t0
+
+let snapshot (#a:Type) (#p:preorder a) (x:pcm_carrier p) : pcm_carrier p =
+  None, snd x
+
+let snapshot_idempotent (#a:Type) (#p:preorder a) (x:pcm_carrier p)
+  : Lemma (snapshot x == snapshot (snapshot x)) = ()
+
+let snapshot_duplicable (#a:Type) (#p:preorder a) (x:pcm_carrier p)
+  : Lemma
+      (requires True)
+      (ensures x `pcm_composable p` snapshot x) = ()
+
+let full_perm_empty_history_compatible (#a:Type) (p:preorder a)
+  : Lemma (compatible (fp_pcm p) (Some full_perm, []) (Some full_perm, [])) =
+  ()
